Removed the useless path computation

src/Reachability.v
@@ -7,6 +7,16 @@ Import ListNotations.
 Open Scope list_scope.
 Implicit Type (σ: Store) (ρ ω: Env) (l: Loc) (L: LocSet).
 
+(* TOCLEAN *)
+Ltac app_eq_nil :=
+  repeat match goal with
+         | H: [] = _ ++ (_ :: _) |- _ => symmetry in H
+         | H: _ ++ (_ :: _) = [] |- _ =>
+             exfalso; apply app_eq_nil in H as [_ H];
+             inverts H
+         end.
+Global Hint Extern 1 => app_eq_nil: core.
+
 
 (** ** Definitions and notations *)
 (** We first define the reachability predicate between two individual locations *)
@@ -26,41 +36,19 @@ Inductive reachability : Store -> Loc -> Loc -> Prop :=
       reachability σ l0 l1 ->
       reachability σ l1 l2 ->
       reachability σ l0 l2.
+Global Hint Constructors reachability: rch.
 
+(** We define the instance for the notation *)
 Global Instance notation_reachability : notation_dash_arrow Store Loc Loc :=
   { dash_arrow_ := reachability }.
-Global Hint Unfold notation_reachability: notations.
+Global Hint Unfold dash_arrow_ notation_reachability: rch.
 
-
-Lemma rch_heap_n : forall l σ, l < dom σ -> σ ⊨ l ⇝ l.
-Proof.
-  autounfold with notations. eauto using reachability.
-Qed.
-
-Lemma rch_step_n : forall l0 l1 C f ω σ,
-    l1 < dom σ ->
-    getObj σ l0 = Some (C, ω) ->
-    getVal ω f = Some l1 ->
-    σ ⊨ l0 ⇝ l1.
-Proof.
-  autounfold with notations. eauto using reachability.
-Qed.
-
-Lemma rch_trans_n : forall l0 l1 l2 σ,
-    σ ⊨ l0 ⇝ l1 ->
-    σ ⊨ l1 ⇝ l2 ->
-    σ ⊨ l0 ⇝ l2.
-Proof.
-  autounfold with notations. eauto using reachability.
-Qed.
-Global Hint Resolve rch_heap_n rch_step_n rch_trans_n : rch.
-
-
+(** Then we define the reachability predicate for sets of locations *)
 Definition reachability_set σ L l := exists l', (l' ∈ L) /\ (σ ⊨ l' ⇝ l).
 Global Instance notation_reachability_set : notation_dash_arrow Store LocSet Loc :=
   { dash_arrow_ := reachability_set }.
 Notation "σ ⊨ { l } ⇝ l'" := (reachability_set σ {l} l')  (at level 60, l at level 98, l' at level 98).
-Global Hint Unfold notation_reachability_set: notations.
+Global Hint Unfold notation_reachability_set: rch.
 
 (** Depending on the temperature of objects we can reach, we have three predicates about the store. Inside a store [σ], a location [l] is said to be:
 - [reachable_cold]: if the location is in the heap (but might point to an object with unitialized fields)
@@ -97,8 +85,9 @@ Global Instance notation_reachability_mode : notation_dash_colon Store Loc Mode 
   }.
 Global Instance notation_reachability_set_mode : notation_dash_colon Store LocSet Mode :=
   { dash_colon_ := fun σ L μ => forall l, l ∈ L -> σ ⊨ l : μ }.
-Global Hint Unfold notation_reachability notation_reachability_set
-       notation_reachability_mode notation_reachability_set_mode: notations.
+
+Global Hint Unfold reachable_cold reachable_cool reachable_hot reachable_warm: rch.
+Global Hint Unfold notation_reachability_mode notation_reachability_set_mode: rch.
 
 (** ** Tactics *)
 
@@ -129,8 +118,9 @@ Lemma reachability_hot:
     σ ⊨ l ⇝ l' ->
     σ ⊨ l': hot.
 Proof.
-  autounfold with notations.
-  unfold reachable_hot; eauto with rch.
+  intros. cbn in *.
+  unfold reachable_hot in *.
+  eauto with rch.
 Qed.
 
 (** Reaching from a singleton is the same as reaching from the only element of the singleton *)
@@ -187,641 +177,322 @@ Lemma reachability_add_env:
 Proof with eauto with rch notations.
   intros σ x C ω l Hx Hobj.
   apply reachability_rev_ind; steps;
-    updates;
-    eauto with rch notations.
+    updates; try solve [right; eauto with rch]...
   destruct_eq (x = l0); subst; updates...
   eapply_anywhere getVal_add; steps...
+  right; split...
 Qed.
 
-(** ** Notions of path into the heap *)
+(** Decidability of reachability *)
 
-(** We define an existential predicate corresponding to the [rch_step] case *)
-Definition reachable_one_step σ l0 l1 :=
-  exists C ω f, getObj σ l0 = (Some (C, ω) : option Obj) /\
-           getVal ω f = Some l1 /\
-           l1 < dom σ.
+Reserved Notation "s ⊨ x ⇝ y ↑ tr" (at level 60, x at level 98, y at level 98, tr at level 98).
+Inductive reachability_trace : Store -> Loc -> Loc -> (list Loc) -> Prop :=
+| rch_t_heap : forall σ l,
+    l < dom σ ->
+    σ ⊨ l ⇝ l ↑ []
+| rch_t_step : forall σ l C ω f l',
+    getObj σ l = Some (C, ω) ->
+    getVal ω f = Some l' ->
+    l' < dom σ ->
+    σ ⊨ l ⇝ l' ↑ []
+| rch_t_trans : forall σ l0 l1 l2 t1 t2,
+    σ ⊨ l0 ⇝ l1 ↑ t1 ->
+    σ ⊨ l1 ⇝ l2 ↑ t2 ->
+    σ ⊨ l0 ⇝ l2 ↑ (t1++l1::t2)
+where "s ⊨ x ⇝ y ↑ tr" := (reachability_trace s x y tr).
+Local Hint Constructors reachability_trace: rch.
 
-Lemma reachable_one_step_reachability :
-  forall σ l0 l1, reachable_one_step σ l0 l1 -> σ ⊨ l0 ⇝ l1.
-Proof.
-  unfold reachable_one_step; steps.
-  eauto with rch notations.
+Lemma rch_iff_rch_tr:
+  forall σ l l',
+    (σ ⊨ l ⇝ l') <-> (exists tr, σ ⊨ l ⇝ l' ↑ tr).
+Proof with (eauto with rch).
+  split; intros.
+  - induction H; flatten; eexists...
+  - destruct H as [tr H].
+    induction H...
 Qed.
-Global Hint Resolve reachable_one_step_reachability : rch.
-Global Hint Extern 1 => eapply_anywhere reachable_one_step_reachability : rch.
+Local Hint Resolve rch_iff_rch_tr: rch.
 
-(** We define the notion of [reachable_path] in σ. The list of points are in reverse order (the head of the list is the end of the path) *)
-Fixpoint reachable_path σ (p: list Loc) {struct p}:=
-  match p with
-  | [] => True
-  | l1::nil => l1 < dom σ
-  | l2::((l1::_) as p') => reachable_one_step σ l1 l2 /\ reachable_path σ p'
-  end.
-
-(** A key notion for scopability proofs is to know if a path contains a given edge *)
-Definition contains_edge p l1 l2 :=
-  exists p1 p2, p = p2 ++ l2::l1::p1.
-
-(** *** Basic properties of paths *)
-(** Transitivity: *)
-Lemma reachable_path_trans:
-  forall σ p1 p2 l,
-    reachable_path σ (p1++[l]) ->
-    reachable_path σ (l::p2) ->
-    reachable_path σ (p1++(l::p2)).
-Proof.
-  induction p1; [steps | intros].
-  simpl in H |- *.
-  repeat (destruct_match; [destruct p1; steps |]).
-  assert (l0 = l2) by (destruct p1; steps); subst.
-  destruct_and.
-  split; eauto.
-  rewrite_back_any.
-  eapply IHp1; eauto; steps.
-Qed.
-
-(** All elements along a path are reachable from the start: *)
-Lemma reachable_path_is_reachable:
-  forall σ p e l,
-    reachable_path σ (e::p) ->
-    List.In l (e::p) ->
-    σ ⊨ l ⇝ e.
-Proof.
-  induction p ; try solve [repeat light ; eauto using rch_heap with notations].
+Lemma rch_tr_implies_rch:
+  forall σ l l' tr,
+    σ ⊨ l ⇝ l' ↑ tr ->
+    σ ⊨ l ⇝ l'.
+Proof with (eauto with rch).
   intros.
-  destruct H0 as [H0 | H0]; subst.
-  + destruct p eqn:P ; repeat light;
-      apply reachable_one_step_reachability, reachability_dom in H0;
-      apply rch_heap; steps.
-  + destruct p eqn:P; [steps; eapply reachable_one_step_reachability; eauto | ].
-    rewrite <- P in *. simpl in *.
-    destruct_and. eauto with rch.
+  eapply rch_iff_rch_tr...
+Qed.
+Local Hint Resolve rch_tr_implies_rch: rch.
+
+Lemma rch_tr_in_rch:
+  forall σ l l' tr l__m,
+    ((σ ⊨ l ⇝ l' ↑ tr) /\ (List.In l__m tr)) <->
+      (exists t0 t1, tr = t0 ++ l__m :: t1 /\
+                  (σ ⊨ l ⇝ l__m ↑ t0) /\
+                  (σ ⊨ l__m ⇝ l' ↑ t1)).
+Proof with (eauto using app_assoc_reverse with rch).
+  split; intros.
+  - destruct H as [H ?].
+    induction H; steps.
+    apply in_app_iff in H0 as [|[|]].
+    + lets (t & t' & ? & ? & ?): IHreachability_trace1 H0.
+      exists t, (t'++l1::t2); subst; splits... rewrite app_assoc_reverse...
+    + subst.
+      exists t1, t2; splits...
+    + lets (t & t' & ? & ? & ?): IHreachability_trace2 H0.
+      exists (t1++l1::t), t'; subst; splits... rewrite app_assoc_reverse...
+  - destruct H as (t0 & t1 & ? & ? & ?). subst.
+    split...
+    apply in_elt.
 Qed.
 
-(** The last element in the path is also reachable: *)
-Lemma reachable_path_last:
-  forall σ s1 s2 p,
-    reachable_path σ (p++[s2;s1]) ->
-    reachable_path σ (p++[s2]).
-Proof.
-  induction p; simpl in *.
-  + unfold reachable_one_step in * ; steps.
-  + repeat (destruct_match; [ apply_anywhere app_eq_nil; steps | ]).
-    assert ( l = l1 ) by (destruct p; steps); steps.
-Qed.
-
-(** Concatenation of paths: *)
-Lemma reachable_path_app:
-  forall σ s1 s2 p1 p2,
-    reachable_path σ (p2++s2::p1++[s1]) ->
-    reachable_path σ (s2::p1++[s1]) /\ reachable_path σ (p2++[s2]).
-Proof.
-  split.
-  + move: H. move: s1 s2 p1.
-    induction p2; simpl.
-    ++ destruct p1; steps.
-    ++ intros. repeat ( destruct_match; [apply_anywhere app_eq_nil; steps |]).
-       repeat rewrite_back_any.
-       steps; eapply_anywhere IHp2; steps.
-  + assert (forall (l:list Loc) p s, reachable_path σ (p++s::l) -> reachable_path σ (p++[s])); eauto.
-    induction l; steps.
-    specialize (IHl (p++[s]) a).
-    eapply reachable_path_last.
-    repeat rewrite <- app_assoc in *.
-    simpl in *; eauto.
-Qed.
-
-(** **** Technical lemma :*)
-Lemma app_exists_last:
-  forall p (x:Loc),
-  exists y p', x::p = p'++[y].
-Proof.
-  induction p; steps.
-  + exists x, ([]:list Loc); steps.
-  + move /(_ a):IHp => IHp. steps.
-    exists y, (x::p'); steps.
-Qed.
-
-(** *** Main equivalence result *)
-Lemma reachable_path_reachability:
-  forall σ (s e: Loc),
-    ((s = e /\ s < dom σ) \/ (**r trivial case *)
-     exists p, reachable_path σ (e :: (p++[s]))) <-> σ ⊨ s ⇝ e. (**r main case if e ≠ s *)
-Proof.
-  split.
-  + intros [[Heq Hdom] | [p Hp]]; subst; eauto with rch notations.
-    generalize dependent e.
-    induction p;
-      repeat light;
-      eauto with rch notations.
-  + induction 1; flatten; eauto; right.
-    ++ eexists []; simpl; unfold reachable_one_step.
-       repeat eexists; eauto using getObj_dom.
-    ++ exists (p++(l1::p0)).
-       rewrite <- app_assoc, app_comm_cons.
-       eauto using reachable_path_trans, app_comm_cons.
-Qed.
-
-(** *** Other results *)
-(** Splitting of paths: *)
-Lemma reachable_path_app2:
-  forall σ s p1 p2,
-    reachable_path σ (p2++s::p1) ->
-    reachable_path σ (p2++[s]).
-Proof.
-  assert (
-      forall σ s s' p1 p2,
-        reachable_path σ (p2 ++ s :: p1++[s']) ->
-        reachable_path σ (p2 ++ [s])
-    ) by repeat steps || eapply_anywhere reachable_path_app.
-  intros; destruct p1 => //.
-  pose proof (app_exists_last p1 l) ; steps.
-  rewrite H1 in H0; eauto.
-Qed.
-
-(** Containing a given edge is decidable: *)
-Lemma contains_edge_dec :
-  forall p l1 l2,
-    contains_edge p l1 l2 \/
-    not (contains_edge p l1 l2).
-Proof.
-  unfold contains_edge. intros.
-  induction p; steps.
-  + right. steps. symmetry in H. apply app_eq_nil in H. steps.
-  + left. exists p1, (a::p2); steps.
-  + destruct_eq (a = l2); subst.
-    ++ (**r a = l2 *)
-      destruct p; steps.
-      +++ right; steps. symmetry in H0. apply app_eq_unit in H0; steps.
-      +++ destruct_eq (l = l1);
-            [ left | right ]; steps;
-              [ eexists p, [] | destruct p2] ;
-              steps; eauto.
-    ++ (**r a ≠ l2 *)
-      right; steps.
-      destruct p2; steps; eauto.
-Qed.
-
-Lemma contains_edge_cons :
-  forall p l l' l0,
-    contains_edge (l0::p) l l' ->
-    l' <> l0 ->
-    contains_edge p l l'.
-Proof.
-  unfold contains_edge; steps.
-  destruct p2; steps; eauto.
-Qed.
-
-(** Combining previous results, we know that if a path contains a given edge [(l1,l2)], then [l1] is reachable from the start: *)
-Lemma reachable_path_split_on_edge:
-  forall σ s p l1 l2,
-    reachable_path σ (p++[s]) ->
-    contains_edge p l1 l2 ->
-    σ ⊨ s ⇝ l1.
-Proof.
-  unfold contains_edge; steps.
-  move: H. move: l1 l2 p1.
-  induction p2; intros; simpl in *.
-  + eapply reachable_path_is_reachable; flatten; eauto.
-    rewrite app_comm_cons. apply in_app_iff; steps.
-  + destruct_match; [apply_anywhere app_eq_nil; steps |].
-    rewrite <- matched in *. flatten; eauto.
-Qed.
-
-(** When the local environment associated with an object is updated, if the updated value was not part of a given path in the updated store, then it was already valid in the un-updated store.  *)
-Lemma contains_edge_assignment :
-  forall σ σ' C ω ω' p f l l',
-    (getObj σ l) = Some (C, ω) ->
-    ω' = [f ↦ l']ω ->
-    σ' = [l ↦ (C, ω')]σ ->
-    not (contains_edge p l l') ->
-    reachable_path σ' p ->
-    reachable_path σ p.
-Proof with (eauto with rch lia).
+Lemma rch_tr_hd_rch:
+  forall σ l l' tr l__m,
+    (σ ⊨ l ⇝ l' ↑ (l__m::tr)) ->
+    (σ ⊨ l ⇝ l__m ↑ []) /\
+      (σ ⊨ l__m ⇝ l' ↑ tr).
+Proof with (eauto using app_assoc_reverse with rch).
   intros.
-  generalize dependent p.
-  induction p as [| l2 p]; intros; simpl; eauto.
-  destruct p as [| l1 p]; [ simpl in *; subst; updates; eauto |].
-  simpl in H3. destruct_and.
-  split.
-  + unfold reachable_one_step in *; flatten; updates.
-    destruct_eq (l = l1); subst; updates.
-    ++ destruct_eq (l2 = l'); subst ;
-         [exfalso; apply H2; eexists p, []  ; steps |].
-       exists C0, ω; repeat split; eauto.
-       destruct_eq (f = f0); subst; updates...
-    ++ repeat eexists...
-  + apply IHp; eauto.
-    intros [p1 [p2 Hedge]].
-    apply H2. exists p1, (l2::p2).
-    rewrite Hedge; eauto.
+  remember (l__m::tr) as T. gen l__m tr.
+  induction H; intros; steps;
+  destruct t1; steps...
+Qed.
+
+Lemma NoDup_app:
+  forall [A: Type] (l l': list A),
+    NoDup (l++l') -> NoDup l /\ NoDup l'.
+Proof with (eauto using NoDup).
+  induction l; simpl; intros...
+  inverts H...
+  apply IHl in H3 as [ ]. split...
+  apply NoDup_cons...
+  intros Hf; apply H2, in_app_iff...
+Qed.
+
+Lemma rch_tr_NoDup:
+  forall σ l l' tr,
+    σ ⊨ l ⇝ l' ↑ tr ->
+    exists tr__nd, (σ ⊨ l ⇝ l' ↑ tr__nd) /\ NoDup tr__nd.
+Proof with (eauto using NoDup with rch).
+  intros. gen l l'.
+  induction tr; intros.
+  - inverts H;
+      exists ([]: list Loc); splits...
+  - lets [ ]: rch_tr_hd_rch H.
+    lets (tr__nd & ? & ?): IHtr H1.
+    destruct (in_dec (PeanoNat.Nat.eq_dec) a tr__nd).
+    + clear IHtr H1 H.
+      pose proof (proj1 (iff_and (rch_tr_in_rch σ a l' tr__nd a)))
+        as (t0 & t1 & ? & ? & ?)...
+      exists (a::t1); split.
+      * replace (a::t1) with ([]++a::t1) by steps...
+      * subst. eapply NoDup_app...
+    + exists (a::tr__nd); split...
+      replace (a::tr__nd) with ([]++a::tr__nd) by steps...
 Qed.
 
 (** A path in an updated store either goes through the new value or was already valid in the un-updated store*)
-Lemma reachable_path_assignment :
-  forall σ σ' C ω ω' p (f l l' : Loc),
-    (getObj σ l) = Some (C, ω) ->
-    ω' = [f ↦ l']ω ->
-    σ' = [l ↦ (C, ω')]σ ->
-    reachable_path σ' p ->
-    contains_edge p l l' \/ reachable_path σ p.
-Proof with (updates; eauto with rch lia).
+Lemma rch_asgn_split :
+  forall σ C ω f l0 l1,
+    getObj σ l0 = Some (C, ω) ->
+    forall l l' σ',
+      σ' ⊨ l ⇝ l' ->
+      σ' = [l0 ↦ (C, [f ↦ l1] ω)] σ ->
+      (σ ⊨ l ⇝ l') \/ ((σ ⊨ l ⇝ l0) /\ (σ ⊨ l1 ⇝ l')).
+Proof with (eauto with rch).
   intros.
-  destruct (contains_edge_dec p l l') as [Hedge | Hedge]; eauto.
-  right.
-  induction p as [| n p ]; eauto.
-  simpl in *.
-  subst.
-  destruct_match... intuition auto.
-  - clear H2. clear H1. unfold reachable_one_step in *; steps...
-    pose proof (getObj_dom _ _ _ H1)...
-    destruct (getObj_Some σ l0 H2) as (C' & ω' & H__getObj).
-    exists C', ω'.
-    destruct_eq (l = l0); subst; updates; cross_rewrites.
-    + destruct_eq (f = f0); subst; updates.
-      * exfalso. apply Hedge.
-           unfold contains_edge.
-           exists l1, ([]: list Loc); steps.
-      * exists f0; splits...
-    + exists f0; splits...
-  - apply H2; clear H2.
-    unfold reachable_one_step, contains_edge in *.
-    intros. flatten.
-    apply Hedge. exists p1, (n::p2). rewrite H2.
-    rewrite app_comm_cons => //.
-Qed.
-
-(** A path is either trivial or contains a first step: *)
-Lemma reachability_first_step:
-  forall σ l1 l2,
-    σ ⊨ l1 ⇝ l2 ->
-    l1 = l2 \/ exists l0, reachable_one_step σ l1 l0.
-Proof.
-  unfold reachable_one_step.
-  intros.
-  induction H; steps.
-  right.  repeat eexists; eauto.
-Qed.
-
-(** We can extract the last edge [(l,l')] of a path: *)
-Lemma contains_edge_last_edge :
-  forall p l l',
-    contains_edge p l l' ->
-    exists p1 p2, p = p1++(l'::l::p2) /\ not (contains_edge p1 l l').
-Proof.
-  induction p as [p IHp] using (induction_ltof1 _ (fun x => length x)); unfold ltof in IHp.
-  intros l l' [p1 [p2 H]].
-  destruct (contains_edge_dec p2 l l').
-  + apply IHp in H0.
-    destruct H0 as [p3 [p4 [H01 H02]]].
-    subst. exists p3 , (p4 ++ l' :: l :: p1) ; split; eauto.
-    repeat rewrite app_comm_cons || rewrite app_assoc => //.
-    subst. rewrite app_length; simpl. Psatz.lia.
-  + exists p2, p1; split; eauto.
-Qed.
-
-(** *** Technical results *)
-Lemma reachability_weaken_assignment :
-(** We define an existential predicate corresponding to the [rch_step] case *)
-  forall (σ σ':Store) C ω ω' (s e: Loc) f l l',
-    (getObj σ l) = Some (C, ω) ->
-    ω' = [f ↦ l']ω ->
-    σ' = [l ↦ (C, ω')]σ ->
-    (l = l') ->
-    σ' ⊨ s ⇝ e ->
-    σ ⊨ s ⇝ e.
-Proof with (updates; eauto with rch lia).
-  intros. move: H3. move: s e.
-  induction 1; subst...
-  destruct_eq (l' = l0); subst ...
-  destruct_eq (f = f0); subst ...
+  (* apply rch_iff_rch_tr in H0 as [tr H0]. *)
+  induction H0; subst; updates...
+  - destruct_eq (l0 = l2); subst; updates...
+    destruct_eq (f = f0); subst; updates...
+    right; split...
+  - intuition auto...
+    + right; split...
+    + right; split...
 Qed.
 
 
-Lemma contains_edge_split:
-  forall y x p p1 p2 (l l': Loc),
-    y :: p ++ [x] = p1 ++ l' :: l :: p2 ->
-    l' = y \/
-    exists p1', p1 = y::p1' /\ y::p++[x] = y::p1'++l'::l::p2.
-Proof.
-  intros.
-  destruct p1; steps.
-  right.
-  exists p1; rewrite_any; steps.
-Qed.
+
+(** ** Assignment results *)
 
 
-Lemma contains_edge_last:
-  forall l l' l0 p1',
-    l <> l' ->
-    contains_edge ((l0 :: p1') ++ [l']) l l' ->
-    contains_edge (l0 :: p1') l l'.
-Proof.
-  unfold contains_edge; steps.
-  destruct p1.
-  - exfalso; eapply_any.
-      eapply (app_inj_tail (p2 ++[l']) (l0::p1')).
-      rewrite app_assoc_reverse; steps.
-  - pose proof (app_exists_last p1 l1); flatten.
-    rewrite H1 in H0.
-    assert (l' = y). {
-      eapply (app_inj_tail (l0::p1') (p2++l'::l::p'));
-        rewrite app_assoc_reverse; eauto. }
-    exists p', p2; steps.
-    eapply app_inv_tail with [y].
-    rewrite app_assoc_reverse; eauto.
-Qed.
+(* Lemma split_or {X} (l : list X) (P Q : X -> Prop) : *)
+(*   (forall x, List.In x l -> (P x \/ Q x)) -> *)
+(*   (exists x, List.In x l /\ P x) \/ (forall x, List.In x l -> Q x). *)
+(* Proof. *)
+(*   induction l; intros. *)
+(*   - right; intros; inversion H0. *)
+(*   - destruct (H a) as [HP | HQ]; [simpl; eauto | | ]. *)
+(*     + left; exists a; simpl; eauto. *)
+(*     + destruct IHl as [[x0 [Hin HP]] | HQ2]; eauto. *)
+(*       * intros y. specialize (H y). *)
+(*         intros. *)
+(*         apply H; simpl; eauto. *)
+(*       * left. exists x0; split; simpl; eauto. *)
+(*       * right; intros. *)
+(*         destruct H0; subst; eauto. *)
+(* Qed. *)
+
+(* Lemma In_tail: *)
+(*   forall (X: Type) (l1 l2: list X) x, *)
+(*     (forall y, List.In y l1 -> List.In y (x::l2)) -> *)
+(*     (List.In x l1) \/ (forall y, List.In y l1 -> List.In y l2). *)
+(* Proof. *)
+(*   intros. *)
+(*   pose proof (split_or l1 (fun y => x=y) (fun y => List.In y l2)). *)
+(*   simpl in H0, H. *)
+(*   apply H0 in H as [[y [H1 H2]] | H1]; subst; eauto. *)
+(* Qed. *)
 
 
-(** Decidability of reachability *)
-Section rch_decidability.
+(* Theorem pigeonhole_principle: *)
+(*   forall (X:Type) (l1 l2:list X), *)
+(*     length l2 < length l1 -> *)
+(*     (forall x, List.In x l1 -> List.In x l2) -> *)
+(*     ~ NoDup l1. *)
+(* Proof. *)
+(*   induction l1 as [|x l1 IH]. *)
+(*   - intros. *)
+(*     inversion H. *)
+(*   - intros. *)
+(*     pose proof (H0 x) as H1; simpl; eauto. *)
+(*     apply in_split in H1 as [l3 [l4 H1]]; simpl; eauto. *)
+(*     specialize (IH (l3++l4)). *)
+(*     subst. *)
+(*     repeat rewrite app_length in H || simpl in H. *)
+(*     repeat rewrite app_length in IH || simpl in IH. *)
+(*     remember (l3++l4) as l2'. *)
+(*     assert (forall y, List.In y l1 -> List.In y (x::l2')). *)
+(*     + intros. subst. *)
+(*       specialize (H0 y). *)
+(*       simpl in *. steps. *)
+(*       rewrite in_app_iff in H0. *)
+(*       rewrite in_app_iff. steps. *)
+(*     + intros HD. inverts HD. *)
+(*       apply In_tail in H1 as [H1 | H1]; eauto using NoDup. *)
+(*       apply IH; eauto with lia. *)
+(* Qed. *)
 
-  Inductive reachability_trace : Store -> Loc -> Loc -> (list Loc) -> Prop :=
-  | rch_t_heap : forall σ l,
-      l < dom σ ->
-      reachability_trace σ l l []
-  | rch_t_step : forall σ l C ω f l',
-      getObj σ l = Some (C, ω) ->
-      getVal ω f = Some l' ->
-      l' < dom σ ->
-      reachability_trace σ l l' []
-  | rch_t_trans : forall σ l0 l1 l2 t1 t2,
-      reachability_trace σ l0 l1 t1 ->
-      reachability_trace σ l1 l2 t2 ->
-      reachability_trace σ l0 l2 (t1++l1::t2).
-  Local Hint Constructors reachability_trace: rch_t.
+(* Import PeanoNat.Nat. *)
 
-  Lemma reachability_trace_reachability:
-    forall σ l l',
-      (σ ⊨ l ⇝ l') <-> (exists p, reachability_trace σ l l' p).
-  Proof with (eauto with rch rch_t).
-    split; intros.
-    - induction H...
-      destruct IHreachability1 as [p1 IH1].
-      destruct IHreachability2 as [p2 IH2].
-      exists (p1++(l1::p2))...
-    - destruct H as [p H].
-      induction H...
-  Qed.
-  Local Hint Resolve reachability_trace_reachability: rch_t.
+(* Fixpoint reachabilityb n σ l l' := *)
+(*   (eqb l l' && ltb l (dom σ)) *)
+(*   || match getObj σ l with *)
+(*     | Some (C, ω) => existsb (eqb l') ω && ltb l' (dom σ) *)
+(*     | None => false *)
+(*     end *)
+(*   || match n with *)
+(*     | 0   => false *)
+(*     | S n => existsb (fun l0 => (reachabilityb n σ l l0) && (reachabilityb n σ l0 l')) (seq 0 (dom σ)) *)
+(*     end. *)
 
-  Lemma reachability_trace_reachability_reverse:
-    forall σ l l' p,
-      reachability_trace σ l l' p -> (σ ⊨ l ⇝ l').
-  Proof.
-    intros.
-    apply reachability_trace_reachability; eauto.
-  Qed.
-  Local Hint Resolve reachability_trace_reachability_reverse: rch_t.
+(* Lemma reachabilityb_monotonicity: *)
+(*   forall n1 n2 σ l l', *)
+(*     n1 <= n2 -> *)
+(*     reachabilityb n1 σ l l' -> *)
+(*     reachabilityb n2 σ l l'. *)
+(* Proof with (bools; eauto with lia). *)
+(*   intros n1 n2. gen n1. *)
+(*   induction n2; simpl in *; intros... *)
+(*   - assert (n1 = 0) by lia; subst. *)
+(*     simpl in H0... *)
+(*   - apply Bool.orb_true_iff. *)
+(*     destruct n1; simpl in *. *)
+(*     + apply Bool.orb_true_iff in H0; steps. *)
+(*     + apply Bool.orb_true_iff in H0 as [|]... *)
+(*       right. *)
+(*       apply existsb_exists in H0 as [x [? ?]]. *)
+(*       apply existsb_exists; exists x; splits... *)
+(*       flatten. *)
+(*       split; eapply IHn2 with (n1 := n1)... *)
+(* Qed. *)
 
-  Lemma reachability_trace_is_reachable:
-    forall σ l l' tr l__m,
-      (reachability_trace σ l l' tr /\
-         List.In l__m tr) <->
-        (exists t0 t1, tr = t0 ++ l__m :: t1 /\
-                    reachability_trace σ l l__m t0 /\
-                    reachability_trace σ l__m l' t1).
-  Proof with (eauto using app_assoc_reverse with rch_t rch).
-    split; intros.
-    - destruct H as [H ?].
-      induction H; steps.
-      apply in_app_iff in H0 as [|[|]].
-      + lets (t & t' & ? & ? & ?): IHreachability_trace1 H0.
-        exists t, (t'++l1::t2); subst; splits... rewrite app_assoc_reverse...
-      + subst.
-        exists t1, t2; splits...
-      + lets (t & t' & ? & ? & ?): IHreachability_trace2 H0.
-        exists (t1++l1::t), t'; subst; splits... rewrite app_assoc_reverse...
-    - destruct H as (t0 & t1 & ? & ? & ?). subst.
-      split...
-      apply in_elt.
-  Qed.
+(* Lemma reachabilityb_reachability: *)
+(*   forall n σ l l', *)
+(*     reachabilityb n σ l l' = true -> σ ⊨ l ⇝ l'. *)
+(* Proof with (bools; eauto with rch lia). *)
+(*   induction n; simpl; intros... *)
+(*   - destruct H as [[[Heq Hlt]|]|]; try discriminate. *)
+(*     + rewrite eqb_eq in Heq. subst. *)
+(*       rewrite ltb_lt in Hlt... *)
+(*     + destruct (getObj σ l) as [[C ω]|] eqn:?; [|discriminate]... *)
+(*       destruct H as [Hex Hlt]. *)
+(*       apply existsb_exists in Hex as [x [ ]]. *)
+(*       rewrite eqb_eq in H0. subst. *)
+(*       apply In_nth_error in H as [f ?]. *)
+(*       apply ltb_lt in Hlt. *)
+(*       eapply rch_step... *)
+(*   - destruct H as [[[Heq Hlt]|]|]. *)
+(*     + rewrite eqb_eq in Heq. subst. *)
+(*       rewrite ltb_lt in Hlt... *)
+(*     + destruct (getObj σ l) as [[C ω]|] eqn:?; [|discriminate]... *)
+(*       destruct H as [Hex Hlt]. *)
+(*       apply existsb_exists in Hex as [x [ ]]. *)
+(*       rewrite eqb_eq in H0. subst. *)
+(*       apply In_nth_error in H as [f ?]. *)
+(*       apply ltb_lt in Hlt. *)
+(*       eapply rch_step... *)
+(*     + apply existsb_exists in H as [l0 [H__l0 ?]]. *)
+(*       apply andb_prop in H as [ ]. *)
+(*       apply rch_trans_n with l0... *)
+(* Qed. *)
+(* Local Hint Resolve reachabilityb_reachability: rch_t. *)
 
-   Lemma reachability_trace_head_reachable:
-    forall σ l l' tr l__m,
-      reachability_trace σ l l' (l__m::tr) ->
-      reachability_trace σ l l__m [] /\
-        reachability_trace σ l__m l' tr.
-  Proof with (eauto using app_assoc_reverse with rch_t rch).
-    intros.
-    remember (l__m::tr) as T. gen l__m tr.
-    induction H; intros... steps. steps.
-    destruct t1; steps...
-  Qed.
+(* Lemma reachability_trace_reachabilityb: *)
+(*   forall σ l l' tr, *)
+(*     reachability_trace σ l l' tr -> reachabilityb (length tr) σ l l'. *)
+(* Proof with (bools; eauto with lia rch_t rch). *)
+(*   intros. *)
+(*   induction H; simpl... *)
+(*   - apply Bool.orb_true_iff. left. *)
+(*     apply Bool.orb_true_iff. left. *)
+(*     apply andb_true_intro; split. *)
+(*     rewrite eqb_eq... *)
+(*     rewrite ltb_lt... *)
+(*   - apply Bool.orb_true_iff. left. *)
+(*     apply Bool.orb_true_iff. right. *)
+(*     rewrite H. *)
+(*     apply andb_true_intro; split. *)
+(*     apply existsb_exists. exists l'; split. *)
+(*     eapply nth_error_In, H0. *)
+(*     rewrite eqb_eq... *)
+(*     rewrite ltb_lt... *)
+(*   - remember (dom t1) as n1. *)
+(*     remember (dom t2) as n2. *)
+(*     rewrite app_length; simpl. *)
+(*     rewrite -Heqn1 -Heqn2 -plus_n_Sm. simpl. *)
+(*     apply Bool.orb_true_intro. right. *)
+(*     apply existsb_exists. exists l1. split; simpl. *)
+(*     + apply in_seq; simpl; split... *)
+(*     + apply andb_true_intro; split; *)
+(*         eapply reachabilityb_monotonicity ; try eassumption... *)
+(* Qed. *)
+(* Local Hint Resolve reachability_trace_reachabilityb : rch_t. *)
 
-  Lemma NoDup_app:
-    forall [A: Type] (l l': list A),
-      NoDup (l++l') -> NoDup l /\ NoDup l'.
-  Proof with (eauto using NoDup).
-    induction l; simpl; intros...
-    inverts H...
-    apply IHl in H3 as [ ]. split...
-    apply NoDup_cons...
-    intros Hf; apply H2, in_app_iff...
-  Qed.
+(* Theorem reachability_dec: *)
+(*   forall σ l l', *)
+(*     {σ ⊨ l ⇝ l'} + {~ σ ⊨ l ⇝ l'}. *)
+(* Proof with (eauto with rch rch_t lia). *)
+(*   intros. *)
+(*   assert (reflect (σ ⊨ l ⇝ l') (reachabilityb (dom σ) σ l l')); [| inverts H; eauto]. *)
+(*   assert ((σ ⊨ l ⇝ l') <-> exists tr, reachability_trace σ l l' tr /\ (length tr <= dom σ)). *)
+(*   - split; intros. *)
+(*     + apply reachability_trace_reachability in H as [tr0 H]. *)
+(*       apply reachability_trace_NoDup in H as [tr [H Hdup]]. *)
+(*       exists tr; split... *)
+(*       assert (dom σ < dom tr \/ dom tr <= dom σ) as [|] by lia... *)
+(*       assert (dom σ = dom (seq 0 (dom σ))); try rewrite seq_length... *)
+(*       rewrite H1 in H0. *)
+(*       eapply pigeonhole_principle in H0. exfalso... *)
+(*       intros. apply in_seq; simpl; split... *)
+(*       pose proof (reachability_trace_is_reachable σ l l' tr x) as [(t0 & t1 & ? & ? & _) _]... *)
+(*     + destruct H as [tr [ ]]... *)
+(*   - destruct (reachabilityb (dom σ) σ l l') eqn:Hb. *)
+(*     + apply Bool.ReflectT... *)
+(*     + apply Bool.ReflectF. *)
+(*       intros Hf. apply H in Hf as [tr [Hf Htr]]. *)
+(*       apply reachability_trace_reachabilityb, reachabilityb_monotonicity with (n2 := dom σ) in Hf... *)
+(* Qed. *)
 
-  Lemma reachability_trace_NoDup:
-    forall σ l l' tr,
-      reachability_trace σ l l' tr ->
-      exists ntr, reachability_trace σ l l' ntr /\ NoDup ntr.
-  Proof with (eauto using NoDup with rch_t).
-    intros. gen l l'.
-    induction tr; intros.
-    - inverts H;
-        exists ([]: list Loc); splits...
-      exfalso. eapply app_cons_not_nil; eauto.
-    - lets [ ]: reachability_trace_head_reachable H.
-      lets (ntr & ? & ?): IHtr H1.
-      destruct (in_dec (PeanoNat.Nat.eq_dec) a ntr).
-      + clear IHtr H1 H.
-        pose proof (proj1 (iff_and (reachability_trace_is_reachable σ a l' ntr a)))
-          as (t0 & t1 & ? & ? & ?)...
-        exists (a::t1); split.
-        * replace (a::t1) with ([]++a::t1) by steps...
-        * subst. eapply NoDup_app...
-      + exists (a::ntr); split...
-        replace (a::ntr) with ([]++a::ntr) by steps...
-  Qed.
+(* End rch_decidability. *)
 
-
-  Lemma split_or {X} (l : list X) (P Q : X -> Prop) :
-    (forall x, List.In x l -> (P x \/ Q x)) ->
-    (exists x, List.In x l /\ P x) \/ (forall x, List.In x l -> Q x).
-  Proof.
-    induction l; intros.
-    + right; intros; inversion H0.
-    + destruct (H a) as [HP | HQ]; [simpl; eauto | | ].
-      ++ left; exists a; simpl; eauto.
-      ++ destruct IHl as [[x0 [Hin HP]] | HQ2]; eauto.
-         +++ intros y. specialize (H y).
-             intros.
-             apply H; simpl; eauto.
-         +++ left. exists x0; split; simpl; eauto.
-         +++ right; intros.
-             destruct H0; subst; eauto.
-  Qed.
-
-  Lemma In_tail:
-    forall (X: Type) (l1 l2: list X) x,
-      (forall y, List.In y l1 -> List.In y (x::l2)) ->
-      (List.In x l1) \/ (forall y, List.In y l1 -> List.In y l2).
-  Proof.
-    intros.
-    pose proof (split_or l1 (fun y => x=y) (fun y => List.In y l2)).
-    simpl in H0, H.
-    apply H0 in H as [[y [H1 H2]] | H1]; subst; eauto.
-  Qed.
-
-
-  Theorem pigeonhole_principle:
-    forall (X:Type) (l1 l2:list X),
-      length l2 < length l1 ->
-      (forall x, List.In x l1 -> List.In x l2) ->
-      ~ NoDup l1.
-  Proof.
-    induction l1 as [|x l1 IH].
-    - intros.
-      inversion H.
-    - intros.
-      pose proof (H0 x) as H1; simpl; eauto.
-      apply in_split in H1 as [l3 [l4 H1]]; simpl; eauto.
-      specialize (IH (l3++l4)).
-      subst.
-      repeat rewrite app_length in H || simpl in H.
-      repeat rewrite app_length in IH || simpl in IH.
-      remember (l3++l4) as l2'.
-      assert (forall y, List.In y l1 -> List.In y (x::l2')).
-      + intros. subst.
-        specialize (H0 y).
-        simpl in *. steps.
-        rewrite in_app_iff in H0.
-        rewrite in_app_iff. steps.
-      + intros HD. inverts HD.
-        apply In_tail in H1 as [H1 | H1]; eauto using NoDup.
-        apply IH; eauto with lia.
-  Qed.
-
-  Import PeanoNat.Nat.
-
-  Fixpoint reachabilityb n σ l l' :=
-    (eqb l l' && ltb l (dom σ))
-    || match getObj σ l with
-      | Some (C, ω) => existsb (eqb l') ω && ltb l' (dom σ)
-      | None => false
-      end
-    || match n with
-      | 0   => false
-      | S n => existsb (fun l0 => (reachabilityb n σ l l0) && (reachabilityb n σ l0 l')) (seq 0 (dom σ))
-      end.
-
-  Lemma reachabilityb_monotonicity:
-    forall n1 n2 σ l l',
-      n1 <= n2 ->
-      reachabilityb n1 σ l l' ->
-      reachabilityb n2 σ l l'.
-  Proof with (bools; eauto with lia).
-    intros n1 n2. gen n1.
-    induction n2; simpl in *; intros...
-    - assert (n1 = 0) by lia; subst.
-      simpl in H0...
-    - apply Bool.orb_true_iff.
-      destruct n1; simpl in *.
-      + apply Bool.orb_true_iff in H0; steps.
-      + apply Bool.orb_true_iff in H0 as [|]...
-        right.
-        apply existsb_exists in H0 as [x [? ?]].
-        apply existsb_exists; exists x; splits...
-        flatten.
-        split; eapply IHn2 with (n1 := n1)...
-  Qed.
-
-  Lemma reachabilityb_reachability:
-    forall n σ l l',
-      reachabilityb n σ l l' = true -> σ ⊨ l ⇝ l'.
-  Proof with (bools; eauto with rch lia).
-    induction n; simpl; intros...
-    - destruct H as [[[Heq Hlt]|]|]; try discriminate.
-      + rewrite eqb_eq in Heq. subst.
-        rewrite ltb_lt in Hlt...
-      + destruct (getObj σ l) as [[C ω]|] eqn:?; [|discriminate]...
-        destruct H as [Hex Hlt].
-        apply existsb_exists in Hex as [x [ ]].
-        rewrite eqb_eq in H0. subst.
-        apply In_nth_error in H as [f ?].
-        apply ltb_lt in Hlt.
-        eapply rch_step...
-    - destruct H as [[[Heq Hlt]|]|].
-      + rewrite eqb_eq in Heq. subst.
-        rewrite ltb_lt in Hlt...
-      + destruct (getObj σ l) as [[C ω]|] eqn:?; [|discriminate]...
-        destruct H as [Hex Hlt].
-        apply existsb_exists in Hex as [x [ ]].
-        rewrite eqb_eq in H0. subst.
-        apply In_nth_error in H as [f ?].
-        apply ltb_lt in Hlt.
-        eapply rch_step...
-      + apply existsb_exists in H as [l0 [H__l0 ?]].
-        apply andb_prop in H as [ ].
-        apply rch_trans_n with l0...
-  Qed.
-  Local Hint Resolve reachabilityb_reachability: rch_t.
-
-  Lemma reachability_trace_reachabilityb:
-    forall σ l l' tr,
-      reachability_trace σ l l' tr -> reachabilityb (length tr) σ l l'.
-  Proof with (bools; eauto with lia rch_t rch).
-    intros.
-    induction H; simpl...
-    - apply Bool.orb_true_iff. left.
-      apply Bool.orb_true_iff. left.
-      apply andb_true_intro; split.
-      rewrite eqb_eq...
-      rewrite ltb_lt...
-    - apply Bool.orb_true_iff. left.
-      apply Bool.orb_true_iff. right.
-      rewrite H.
-      apply andb_true_intro; split.
-      apply existsb_exists. exists l'; split.
-      eapply nth_error_In, H0.
-      rewrite eqb_eq...
-      rewrite ltb_lt...
-    - remember (dom t1) as n1.
-      remember (dom t2) as n2.
-      rewrite app_length; simpl.
-      rewrite -Heqn1 -Heqn2 -plus_n_Sm. simpl.
-      apply Bool.orb_true_intro. right.
-      apply existsb_exists. exists l1. split; simpl.
-      + apply in_seq; simpl; split...
-      + apply andb_true_intro; split;
-          eapply reachabilityb_monotonicity ; try eassumption...
-  Qed.
-  Local Hint Resolve reachability_trace_reachabilityb : rch_t.
-
-  Theorem reachability_dec:
-    forall σ l l',
-      {σ ⊨ l ⇝ l'} + {~ σ ⊨ l ⇝ l'}.
-  Proof with (eauto with rch rch_t lia).
-    intros.
-    assert (reflect (σ ⊨ l ⇝ l') (reachabilityb (dom σ) σ l l')); [| inverts H; eauto].
-    assert ((σ ⊨ l ⇝ l') <-> exists tr, reachability_trace σ l l' tr /\ (length tr <= dom σ)).
-    - split; intros.
-      + apply reachability_trace_reachability in H as [tr0 H].
-        apply reachability_trace_NoDup in H as [tr [H Hdup]].
-        exists tr; split...
-        assert (dom σ < dom tr \/ dom tr <= dom σ) as [|] by lia...
-        assert (dom σ = dom (seq 0 (dom σ))); try rewrite seq_length...
-        rewrite H1 in H0.
-        eapply pigeonhole_principle in H0. exfalso...
-        intros. apply in_seq; simpl; split...
-        pose proof (reachability_trace_is_reachable σ l l' tr x) as [(t0 & t1 & ? & ? & _) _]...
-      + destruct H as [tr [ ]]...
-    - destruct (reachabilityb (dom σ) σ l l') eqn:Hb.
-      + apply Bool.ReflectT...
-      + apply Bool.ReflectF.
-        intros Hf. apply H in Hf as [tr [Hf Htr]].
-        apply reachability_trace_reachabilityb, reachabilityb_monotonicity with (n2 := dom σ) in Hf...
-  Qed.
-
-End rch_decidability.
-
-Check reachability_dec.
+(* Check reachability_dec. *)
